> Prove that Fib(_n_) is the closest integer to 𝜙ⁿ/√5, where 𝜙 = (1 + √5)/2. Hint: Let 𝜓 = (1 - √5)/2.
> Use induction and the definition of the Fibonacci numbers to prove that Fib(_n_) = (𝜙ⁿ - 𝜓ⁿ)/√5.

### Base Step
```
Fib(0) = (𝜙⁰ - 𝜓⁰) / √5 = 0
```

Show that Fib(_n_) = (𝜙ⁿ - 𝜓ⁿ)/√5 for _n_ = 1.

```
Fib(1) = (𝜙¹ - 𝜓¹) / √5
       = ((1 + √5)/2 - (1 - √5)/2) / √5
       = (1 + √5 - 1 + √5) / (2 * √5)
       = 2√5 / 2√5 = 1
```
          
### Inductive Step
Assuming Fib(_n_) = (𝜙ⁿ - 𝜓ⁿ)/√5 holds for _n_,
Show that Fib(_n_ + 1) = (𝜙ⁿ⁺¹ - 𝜓ⁿ⁺¹)/√5.

```
We know that Fib(n) = Fib(n - 1) + Fib(n - 2)
Assuming Fib(n) = (𝜙ⁿ - 𝜓ⁿ)/√5, it follows that 
     Fib(n - 1) = (𝜙ⁿ - 𝜓ⁿ)/√5 - Fib(n - 2)

We know that Fib(n + 1) = Fib(n) + Fib(n - 1)
                        = (𝜙ⁿ - 𝜓ⁿ)/√5 + Fib(n - 1)
                        = (𝜙ⁿ - 𝜓ⁿ)/√5 + (𝜙ⁿ - 𝜓ⁿ)/√5 - Fib(n - 2)
                        = 2(𝜙ⁿ - 𝜓ⁿ)/√5 - Fib(n - 2)
                        = ...
```
```
Fib(_n_ + 1) = (𝜙ⁿ⁺¹ - 𝜓ⁿ⁺¹)/√5
             = (𝜙ⁿ𝜙 - 𝜓ⁿ𝜓)/√5
             = (𝜙ⁿ𝜙)/√5 - (𝜓ⁿ𝜓)/√5
             = (𝜙ⁿ(1 + √5)/2)/√5 - (𝜓ⁿ(1 - √5)/2)/√5
             = (𝜙ⁿ(1 + √5))/2√5 - (𝜓ⁿ(1 - √5))/2√5
             = ((𝜙ⁿ(1 + √5)) - (𝜓ⁿ(1 - √5)))/2√5
             = ((𝜙ⁿ + 𝜙ⁿ√5) - (𝜓ⁿ - 𝜓ⁿ√5))/2√5
             = (𝜙ⁿ + 𝜙ⁿ√5)/2√5 - (𝜓ⁿ - 𝜓ⁿ√5)/2√5
             = 𝜙ⁿ/2√5 + 𝜙ⁿ√5/2√5 - 𝜓ⁿ2√5 - 𝜓ⁿ√5/2√5
             = 𝜙ⁿ/2√5 + 2𝜙ⁿ - (𝜓ⁿ2√5 + 2𝜓ⁿ)

                        
...

```


